mise a jour interface coq/caml

coq/api.v
@@ -3,37 +3,37 @@ Require Import String.
 
 Definition mlSort := string.
 
-Record mlVariable := {
-  mlVarName: string;
-  mlVarSort: mlSort;
+Record variable :=make_variable {
+  var_name: string;
+  var_sort: mlSort;
 }.
 
-Record mlConstant := {
-  mlCstName: string;
-  mlCstSort: mlSort;
+Record constant := make_constant {
+  cst_name: string;
+  cst_sort: mlSort;
 }.
 
-Record mlRelation := {
-  mlRelName: string;
-  mlRelArity : list mlSort;
+Record relation := make_relation {
+  rel_name: string;
+  rel_profile : list mlSort;
 }.
 
 Inductive mlIdent :=
 | MLS (s: mlSort)
-| MLV (v: mlVariable)
-| MLC (c: mlConstant)
-| MLR (r: mlRelation).
+| MLV (v: variable)
+| MLC (c: constant)
+| MLR (r: relation).
 
 Definition isMLSort id := match id with MLS _ => True | _ => False end.
-Definition isMLVar id := match id with MLV _ => True | _ => False end.
-Definition isMLCst id := match id with MLC _ => True | _ => False end.
+Definition isVar id := match id with MLV _ => True | _ => False end.
+Definition isCst id := match id with MLC _ => True | _ => False end.
 Definition isMLRel id := match id with MLR _ => True | _ => False end.
 Definition getMLSort id : isMLSort id -> _ :=
   match id return isMLSort id -> _ with MLS s => fun h => s | _ => fun h => match h with end end.
-Definition getMLVar id : isMLVar id -> _ :=
-  match id return isMLVar id -> _ with MLV v => fun h => v | _ => fun h => match h with end end.
-Definition getMLCst id : isMLCst id -> _ :=
-  match id return isMLCst id -> _ with MLC c => fun h => c | _ => fun h => match h with end end.
+Definition getVar id : isVar id -> _ :=
+  match id return isVar id -> _ with MLV v => fun h => v | _ => fun h => match h with end end.
+Definition getCst id : isCst id -> _ :=
+  match id return isCst id -> _ with MLC c => fun h => c | _ => fun h => match h with end end.
 Definition getMLRel id : isMLRel id -> _ :=
   match id return isMLRel id -> _ with MLR r => fun h => r | _ => fun h => match h with end end.
   
@@ -41,11 +41,11 @@ Lemma isMLSortDec id : { isMLSort id } + { not (isMLSort id) }.
 Proof.
   destruct id; simpl; try (left; simpl; now auto); right; intro; tauto.
 Defined.
-Lemma isMLVarDec id : { isMLVar id } + { not (isMLVar id) }.
+Lemma isVarDec id : { isVar id } + { not (isVar id) }.
 Proof.
   destruct id; simpl; try (left; simpl; now auto); right; intro; tauto.
 Defined.
-Lemma isMLCstDec id : { isMLCst id } + { not (isMLCst id) }.
+Lemma isCstDec id : { isCst id } + { not (isCst id) }.
 Proof.
   destruct id; simpl; try (left; simpl; now auto); right; intro; tauto.
 Defined.
@@ -54,73 +54,71 @@ Proof.
   destruct id; simpl; try (left; simpl; now auto); right; intro; tauto.
 Defined.
 
-Inductive mlTerm : Type :=
-  MLVar (v: mlVariable)
-| MLCst (c: mlConstant).
+Inductive term : Type :=
+  Var (v: variable)
+| Cst (c: constant).
 
-Definition mlTermSort (tm: mlTerm): mlSort :=
+Definition termSort (tm: term): mlSort :=
   match tm with
-    MLVar v => mlVarSort v
-  | MLCst c => mlCstSort c
+    Var v => var_sort v
+  | Cst c => cst_sort c
   end.
 
-Definition isMLLit (r: mlRelation) (args: list mlTerm): Prop := 
-  mlRelArity r = List.map mlTermSort args.
+Definition isMLLit (r: relation) (args: list term): Prop := 
+  rel_profile r = List.map termSort args.
 
-Inductive mlLiteral: Type :=
-  MLPApp (nx: nat) (r: string) (args: list mlTerm).
+Inductive literal: Type :=
+| Pos_app (nx: nat) (r: string) (args: list term)
+| Neg_app (nx: nat) (r: string) (args: list term)
+| Eq (t1: term) (t2: term)
+| Not_eq (t1: term) (t2: term).
 
-Inductive mlAtom: Type :=
-| MLLiteral (lt: mlLiteral)
-| MLNLiteral (lt: mlLiteral)
-| MLEq (t1: mlTerm) (t2: mlTerm)
-| MLNEq (t1: mlTerm) (t2: mlTerm).
+Inductive formula: Type :=
+  True: formula
+| False: formula
+| Lit: literal -> formula
+| And: formula -> formula -> formula 
+| Or: formula -> formula -> formula
+| Exists: variable -> formula -> formula
+| All: variable -> formula -> formula
+| F: formula -> formula
+| G: formula -> formula.
 
-Inductive mlFormula: Type :=
-  MLFTrue: mlFormula
-| MLFFalse: mlFormula
-| MLAtom: mlAtom -> mlFormula
-| MLAnd: mlFormula -> mlFormula -> mlFormula 
-| MLOr: mlFormula -> mlFormula -> mlFormula
-| MLEx: mlVariable -> mlFormula -> mlFormula
-| MLAll: mlVariable -> mlFormula -> mlFormula
-| MLF: mlFormula -> mlFormula
-| MLG: mlFormula -> mlFormula.
+Definition ev_modification := list term.
 
-Definition mlEvMod := list mlTerm.
-
-Record mlEvModify := {
-  mlModRel: mlRelation;
-  mlModMods : list mlEvMod;
+Record ev_modify := make_ev_modify {
+  mod_rel: relation;
+  mod_mods : list ev_modification;
 }.
 
-Record mlEvent := {
-  mlEvName : string;
-  mlEvArgs : list mlVariable;
-  mlEvBody : mlFormula;
-  mlEvModifies : list mlEvModify;
+Record event := make_event {
+  ev_name : string;
+  ev_args : list variable;
+  ev_body : formula;
+  ev_modificationifies : list ev_modify;
 }.
 
 Inductive mlUsing :=
   TEA: mlUsing (* transfo Ex -> Alll avec intro E *)
-| TTC: mlRelation -> mlVariable -> mlFormula -> mlUsing (* transitive closure *)
-| TFC: (mlEvent -> mlFormula) -> mlUsing. (* frame condition *)
+| TTC: relation -> variable -> formula -> mlUsing (* transitive closure *)
+| TFC: (event -> formula) -> mlUsing. (* frame condition *)
 
-Record mlCheck := {
-  mlChkName: string;
-  mlChkBody: mlFormula;
-  mlChkAssumes: mlFormula;
-  mlChkUsing: mlUsing;
+Record check := make_check {
+  chk_name: string;
+  chk_body: formula;
+  chk_assuming: formula;
+  chk_using: mlUsing;
 }.
 
-Record mlPath := {
-  mlTC : mlRelation;
-  mlBase : mlRelation;
+Record path := make_path {
+  tc : relation;
+  base : relation;
+  between : option relation
 }.
 
-Record mlModel := {
-  mlAxioms : list mlFormula;
-  mlEvents : list mlEvent;
-  mlClosures : list mlPath;
-  mlCheckWith : mlCheck;
+Record model := make_model {
+  axioms : list formula;
+  events : list event;
+  closures : list path;
+  checkWith : check;
 }.
