coq/api2coq.v
@@ -6,9 +6,9 @@ Require Import ProofIrrelevance.
 Require Import Init.Logic.
 Import  EqNotations.
 
-Require Import api.
-Require Import mlUtils.
-Require Import foltl.
+Require api.
+Require mlUtils.
+Require foltl.
 Require Import finite.
 Require Import dec.
 Require Import utils.
@@ -17,13 +17,13 @@ Instance StrDec : EqDec := {| eq_dec := string_dec |}.
 Instance NatDec : EqDec := {| eq_dec := Coq.Arith.PeanoNat.Nat.eq_dec |}.
 
 Section ML2Coq.
-Variable mdl : mlModel.
+Variable mdl : api.model.
 
-Definition mlSorts2Sort : SortT := asFinite (mlSorts mdl).
-Definition mlSort2Sort (s: mlSort) (h: List.In s (mlSorts mdl)) : mlSorts2Sort :=
+Definition mlSorts2Sort : foltl.SortT := asFinite (mlUtils.mlSorts mdl).
+Definition mlSort2Sort (s: api.mlSort) (h: List.In s (mlUtils.mlSorts mdl)) : mlSorts2Sort :=
  exist _ s h.
 
-Instance mlVariableDec: @EqDec mlVariable.
+Instance variableDec: @EqDec api.variable.
 Proof.
   split; repeat intro.
   destruct x as [v1 h1]; destruct y as [v2 h2].
@@ -40,7 +40,7 @@ Proof.
   apply (n H0).
 Defined.
 
-Instance mlConstantDec: @EqDec mlConstant.
+Instance constantDec: @EqDec api.constant.
 Proof.
   split; repeat intro.
   destruct x as [v1 h1]; destruct y as [v2 h2].
@@ -57,7 +57,7 @@ Proof.
   apply (n H0).
 Defined.
 
-Instance mlRelationDec: @EqDec mlRelation.
+Instance relationDec: @EqDec api.relation.
 Proof.
   split; repeat intro.
   destruct x as [v1 h1]; destruct y as [v2 h2].
@@ -74,136 +74,133 @@ Proof.
   apply (n H0).
 Defined.
 
-Program Definition coqSig : Sig := {|
-  Sort := mlSorts2Sort;
-  variable s := asFinite (mlVariables mdl (proj1_sig s));
-  constant s := asFinite (mlConstants mdl (proj1_sig s));
-  predicate := asFinite (mlRelations mdl);
-  pr_arity p := List.length (mlRelArity (proj1_sig p));
-  pr_args p i := exist _ (fnth (mlRelArity (proj1_sig p)) i) _
+Program Definition coqSig : foltl.Sig := {|
+  foltl.Sort := mlSorts2Sort;
+  foltl.variable s := asFinite (mlUtils.variables mdl (proj1_sig s));
+  foltl.constant s := asFinite (mlUtils.constants mdl (proj1_sig s));
+  foltl.predicate := asFinite (mlUtils.relations mdl);
+  foltl.pr_arity p := List.length (api.rel_profile (proj1_sig p));
+  foltl.pr_args p i := exist _ (fnth (api.rel_profile (proj1_sig p)) i) _
 |}.
 Next Obligation.
   destruct p as [r h]; simpl in *.
-  apply (mlSortOfRelAritiesIn mdl r h).
+  apply (mlUtils.mlSortOfRelAritiesIn mdl r h).
   apply fnth_In.
 Defined.
 
-Definition mlSortOfVar v h: Sort (Sig:=coqSig) :=
-  (mlSort2Sort (mlVarSort v) (mlSortOfVarsIn mdl v h)).
+Definition mlSortOfVar v h: foltl.Sort (Sig:=coqSig) :=
+  (mlSort2Sort (api.var_sort v) (mlUtils.mlSortOfVarsIn mdl v h)).
 
-Definition mlSortOfCst v h: Sort (Sig:=coqSig) :=
-  (mlSort2Sort (mlCstSort v) (mlSortOfCstsIn mdl v h)).
+Definition mlSortOfCst v h: foltl.Sort (Sig:=coqSig) :=
+  (mlSort2Sort (api.cst_sort v) (mlUtils.mlSortOfCstsIn mdl v h)).
 
-Program Definition mlSortOfTerm t: List.incl (mlTermIds t) (mlModelIds mdl) -> Sort (Sig:=coqSig) := 
-  match t return List.incl (mlTermIds t) (mlModelIds mdl) -> _ with
-    MLVar v => fun h => mlSortOfVar v _
-  | MLCst c => fun h => mlSortOfCst c _
+Program Definition mlSortOfTerm t: List.incl (mlUtils.termIds t) (mlUtils.modelIds mdl) -> foltl.Sort (Sig:=coqSig) := 
+  match t return List.incl (mlUtils.termIds t) (mlUtils.modelIds mdl) -> _ with
+    api.Var v => fun h => mlSortOfVar v _
+  | api.Cst c => fun h => mlSortOfCst c _
   end.
 Next Obligation.
-  generalize (h (MLV v)); clear h; intro h.
-  assert (In (MLV v) (mlVarIds v)) by (unfold mlVarIds; simpl; tauto).
+  generalize (h (api.MLV v)); clear h; intro h.
+  assert (In (api.MLV v) (mlUtils.mlVarIds v)) by (unfold mlUtils.mlVarIds; simpl; tauto).
   apply h in H; clear h.
-  unfold mlAllVariables.
-  apply (imap_filter_In_intro _ _ isMLVarDec (mlModelIds mdl)
-   (fun (v0 : mlIdent) (h1 : isMLVar v0) (_ : In v0 (mlModelIds mdl))
-      => getMLVar v0 h1) (MLV v) I H).
+  unfold mlUtils.mlAllVariables.
+  apply (imap_filter_In_intro _ _ api.isVarDec (mlUtils.modelIds mdl)
+   (fun (v0 : api.mlIdent) (h1 : api.isVar v0) (_ : In v0 (mlUtils.modelIds mdl))
+      => api.getVar v0 h1) (api.MLV v) I H).
 Qed.
 Next Obligation.
-  generalize (h (MLC c)); clear h; intro h.
-  assert (In (MLC c) (mlCstIds c)) by (unfold mlCstIds; simpl; tauto).
+  generalize (h (api.MLC c)); clear h; intro h.
+  assert (In (api.MLC c) (mlUtils.mlCstIds c)) by (unfold mlUtils.mlCstIds; simpl; tauto).
   apply h in H; clear h.
-  unfold mlAllConstants.
-  apply (imap_filter_In_intro _ _ isMLCstDec (mlModelIds mdl)
-   (fun (v0 : mlIdent) (h1 : isMLCst v0) (_ : In v0 (mlModelIds mdl))
-      => getMLCst v0 h1) (MLC c) I H).
+  unfold mlUtils.mlAllConstants.
+  apply (imap_filter_In_intro _ _ api.isCstDec (mlUtils.modelIds mdl)
+   (fun (v0 : api.mlIdent) (h1 : api.isCst v0) (_ : In v0 (mlUtils.modelIds mdl))
+      => api.getCst v0 h1) (api.MLC c) I H).
 Qed.
 
 Lemma mlSortOfTerm_mlSort2Sort: forall t h i,
-  mlSortOfTerm t h = mlSort2Sort (mlTermSort t) i.
+  mlSortOfTerm t h = mlSort2Sort (api.termSort t) i.
 Proof.
   intros.
   destruct t; simpl.
   destruct v as [v h1].
-  unfold mlTermSort, mlSortOfVar, mlSort2Sort in *; simpl in *.
+  unfold api.termSort, mlSortOfVar, mlSort2Sort in *; simpl in *.
   f_equal.
   apply proof_irrelevance.
 
   destruct c as [c h1].
-  unfold mlTermSort, mlSortOfCst, mlSort2Sort in *; simpl in *.
+  unfold api.termSort, mlSortOfCst, mlSort2Sort in *; simpl in *.
   f_equal.
   apply proof_irrelevance.
 Qed.
 
-Program Definition mlVar2Var (v: mlVariable) h: variable (Sig:=coqSig) (mlSortOfVar v h) :=
+Program Definition mlVar2Var (v: api.variable) h: foltl.variable (Sig:=coqSig) (mlSortOfVar v h) :=
   exist _ v _.
 Next Obligation.
-  unfold mlVariables.
+  unfold mlUtils.variables.
   apply filter_In.
   split; auto.
-  destruct (string_dec (mlVarSort v) (mlVarSort v)); tauto.
+  destruct (string_dec (api.var_sort v) (api.var_sort v)); tauto.
 Qed.
 
-Program Definition mlCst2Cst (c: mlConstant) h: constant (Sig:=coqSig) (mlSortOfCst c h) :=
+Program Definition mlCst2Cst (c: api.constant) h: foltl.constant (Sig:=coqSig) (mlSortOfCst c h) :=
   exist _ c _.
 Next Obligation.
-  unfold mlConstants.
+  unfold mlUtils.constants.
   apply filter_In.
   split; auto.
-  destruct (string_dec (mlCstSort c) (mlCstSort c)); tauto.
+  destruct (string_dec (api.cst_sort c) (api.cst_sort c)); tauto.
 Qed.
 
-Definition mlTerm2Term t: forall h, term coqSig (mlSortOfTerm t h) :=
-  match t return forall h, term coqSig (mlSortOfTerm t h) with
-    MLVar v => fun h => Var coqSig _ (mlVar2Var v (mlSortOfTerm_obligation_1 v h))
-  | MLCst c => fun h => Cst coqSig _ (mlCst2Cst c (mlSortOfTerm_obligation_2 c h))
+Definition term2Term t: forall h, foltl.term coqSig (mlSortOfTerm t h) :=
+  match t return forall h, foltl.term coqSig (mlSortOfTerm t h) with
+    api.Var v => fun h => foltl.Var coqSig _ (mlVar2Var v (mlSortOfTerm_obligation_1 v h))
+  | api.Cst c => fun h => foltl.Cst coqSig _ (mlCst2Cst c (mlSortOfTerm_obligation_2 c h))
   end.
 
-Definition mlRelation2Pred p (h: List.In p (mlRelations mdl)): predicate (Sig:=coqSig) :=
+Definition relation2Pred p (h: List.In p (mlUtils.relations mdl)): foltl.predicate (Sig:=coqSig) :=
   exist _ p h.
 
-Program Definition mlLiteral2Literal l:  List.incl (mlLitIds l) (mlModelIds mdl) -> literal coqSig :=
-  match l return List.incl(mlLitIds l) (mlModelIds mdl) -> literal coqSig with
-    MLPApp x p al => fun h =>
-      let r := {| mlRelName := p; mlRelArity := List.map mlTermSort al |} in
-      PApp coqSig x (mlRelation2Pred r _) 
-        (fun i => mlTerm2Term (fnth al i) _)
-  end.
+Program Definition mlLiteral2Literal x p al (h: List.incl (mlUtils.mlLitIds p al) (mlUtils.modelIds mdl)): foltl.literal coqSig :=
+    let r := {| api.rel_name := p; api.rel_profile := List.map api.termSort al |} in
+      foltl.PApp coqSig x (relation2Pred r _) 
+        (fun i => term2Term (fnth al i) _).
 Next Obligation.
-  revert h; set (r:={| mlRelName := p; mlRelArity := map mlTermSort al |}); intros.
-  unfold mlRelations.
-  unfold mlRelIds in h.
-  generalize (h (MLR r) (or_introl eq_refl)); clear h; intro h.
-  apply (imap_filter_In_intro _ _ isMLRelDec (mlModelIds mdl)
-   (fun (v0 : mlIdent) (h1 : isMLRel v0) (_ : In v0 (mlModelIds mdl))
-      => getMLRel v0 h1) (MLR r) I h).
+  revert h; set (r:={| api.rel_name := p; api.rel_profile := map api.termSort al |}); intros.
+  unfold mlUtils.relations.
+  unfold mlUtils.mlRelIds in h.
+  generalize (h (api.MLR r) (or_introl eq_refl)); clear h; intro h.
+  apply (imap_filter_In_intro _ _ api.isMLRelDec (mlUtils.modelIds mdl)
+   (fun (v0 : api.mlIdent) (h1 : api.isMLRel v0) (_ : In v0 (mlUtils.modelIds mdl))
+      => api.getMLRel v0 h1) (api.MLR r) I h).
 Qed.
 Next Obligation.
   apply map_length.
 Qed.
 Next Obligation.
-  generalize (mlLiteral2Literal_obligation_2 x p al h).
-  generalize (mlLiteral2Literal_obligation_1 x p al h); intros.
+  generalize (mlLiteral2Literal_obligation_2 p al h).
+  generalize (mlLiteral2Literal_obligation_1 p al h); intros.
   apply incl_cons_inv in h; apply proj2 in h.
   apply incl_app_inv in h; apply proj2 in h.
   revert h; apply incl_tran.
-  unfold mlRelation2Pred in e; simpl in e.
+  unfold relation2Pred in e; simpl in e.
   revert i; rewrite e; intro; simpl.
-  apply incl_concat_r_intro with (i := (rew [Fin.t] (eq_sym (map_length mlTermIds al)) in i)).
+  apply incl_concat_r_intro with (i := (rew [Fin.t] (eq_sym (map_length mlUtils.termIds al)) in i)).
   rewrite fnth_map.
-  generalize (map_length mlTermIds al); intro.
+  generalize (map_length mlUtils.termIds al); intro.
   revert i i0 e; rewrite e0; intros; simpl.
   apply incl_refl.
 Qed.
 Next Obligation.
-  generalize (mlLiteral2Literal_obligation_3 x p al h i).
-  generalize (mlLiteral2Literal_obligation_2 x p al h).
-  generalize (mlLiteral2Literal_obligation_1 x p al h); intros.
+  generalize (mlLiteral2Literal_obligation_3 p al h i).
+  generalize (mlLiteral2Literal_obligation_2 p al h).
+  generalize (mlLiteral2Literal_obligation_1 p al h); intros.
   simpl in e.
-  generalize (mlSortOfRelAritiesIn mdl {| mlRelName := p; mlRelArity := map mlTermSort al |} i0
-     (fnth (map mlTermSort al) i) (fnth_In (map mlTermSort al) i)); intro.
+  generalize (mlUtils.mlSortOfRelAritiesIn mdl {| api.rel_name := p; api.rel_profile := map api.termSort al |} i0
+     (fnth (map api.termSort al) i) (fnth_In (map api.termSort al) i)); intro.
   simpl in i1.
   revert i2; rewrite fnth_map; intros.
-  revert i2; generalize (map_length mlTermSort al); intros.
+  revert i2; generalize (map_length api.termSort al); intros.
   revert i2; rewrite (proof_irrelevance _ e0 e); clear e0; intro.
   change (fun H => Fin.t H) with Fin.t in *.
   revert i1 i2; generalize (fnth al (rew [Fin.t] e in i)); intros.
@@ -211,67 +208,67 @@ Next Obligation.
   reflexivity.
 Qed.
 
-Lemma mlTermSortInIds: forall t, In (MLS (mlTermSort t)) (mlTermIds t).
+Lemma termSortInIds: forall t, In (api.MLS (api.termSort t)) (mlUtils.termIds t).
 Proof.
   intros.
   destruct t; simpl; tauto.
 Qed.
 
-Lemma mlTermIn2mlTermSortIn: forall t,
-  incl (mlTermIds t) (mlModelIds mdl) -> In (mlTermSort t) (mlSorts mdl).
+Lemma termIn2termSortIn: forall t,
+  incl (mlUtils.termIds t) (mlUtils.modelIds mdl) -> In (api.termSort t) (mlUtils.mlSorts mdl).
 Proof.
   intros.
-  generalize (mlTermSortInIds t); intro.
+  generalize (termSortInIds t); intro.
   apply H in H0; clear H.
-  apply (imap_filter_In_intro _ _ isMLSortDec (mlModelIds mdl)
-   (fun (v0 : mlIdent) (h1 : isMLSort v0) (_ : In v0 (mlModelIds mdl))
-      => getMLSort v0 h1) (MLS _) I H0).  
+  apply (imap_filter_In_intro _ _ api.isMLSortDec (mlUtils.modelIds mdl)
+   (fun (v0 : api.mlIdent) (h1 : api.isMLSort v0) (_ : In v0 (mlUtils.modelIds mdl))
+      => api.getMLSort v0 h1) (api.MLS _) I H0).  
 Qed.
 
-Program Definition mlAtom2Atom a : List.incl (mlAtomIds a) (mlModelIds mdl) -> formula coqSig :=
-  match a return List.incl (mlAtomIds a) (mlModelIds mdl) -> formula coqSig with
-  | MLLiteral l => fun h => Atom _ (Literal coqSig (mlLiteral2Literal l h))
-  | MLNLiteral l => fun h => Atom _ (NLiteral coqSig (mlLiteral2Literal l h))
-  | MLEq t1 t2 => fun h => let (h1,h2) := incl_app_inv _ _ h in
-    match (string_dec (mlTermSort t1) (mlTermSort t2)) with
-      left e => Atom coqSig (Eq coqSig (mlSortOfTerm t1 _) (mlTerm2Term t1 _) (mlTerm2Term t2 _))
-    | right _ => FFalse coqSig
+Program Definition literal2Atom a : List.incl (mlUtils.mlAtomIds a) (mlUtils.modelIds mdl) -> foltl.formula coqSig :=
+  match a return List.incl (mlUtils.mlAtomIds a) (mlUtils.modelIds mdl) -> foltl.formula coqSig with
+  | api.Pos_app x r args => fun h => foltl.Atom _ (foltl.Literal coqSig (mlLiteral2Literal x r args h))
+  | api.Neg_app x r args => fun h => foltl.Atom _ (foltl.NLiteral coqSig (mlLiteral2Literal x r args h))
+  | api.Eq t1 t2 => fun h => let (h1,h2) := incl_app_inv _ _ h in
+    match (string_dec (api.termSort t1) (api.termSort t2)) with
+      left e => foltl.Atom coqSig (foltl.Eq coqSig (mlSortOfTerm t1 _) (term2Term t1 _) (term2Term t2 _))
+    | right _ => foltl.FFalse coqSig
     end
-  | MLNEq t1 t2 => fun h => let (h1,h2) := incl_app_inv _ _ h in
-    match (string_dec (mlTermSort t1) (mlTermSort t2)) with
-      left e => Atom coqSig (NEq coqSig (mlSortOfTerm t1 _) (mlTerm2Term t1 _) (mlTerm2Term t2 _))
-    | right _ => FTrue coqSig
+  | api.Not_eq t1 t2 => fun h => let (h1,h2) := incl_app_inv _ _ h in
+    match (string_dec (api.termSort t1) (api.termSort t2)) with
+      left e => foltl.Atom coqSig (foltl.NEq coqSig (mlSortOfTerm t1 _) (term2Term t1 _) (term2Term t2 _))
+    | right _ => foltl.FTrue coqSig
     end
   end.
 Next Obligation.
-  rewrite mlSortOfTerm_mlSort2Sort with (i:=mlTermIn2mlTermSortIn _ h1).
-  rewrite mlSortOfTerm_mlSort2Sort with (i:=mlTermIn2mlTermSortIn _ h2).
-  generalize (mlTermIn2mlTermSortIn t1 h1); rewrite e; intro.
+  rewrite mlSortOfTerm_mlSort2Sort with (i:=termIn2termSortIn _ h1).
+  rewrite mlSortOfTerm_mlSort2Sort with (i:=termIn2termSortIn _ h2).
+  generalize (termIn2termSortIn t1 h1); rewrite e; intro.
   f_equal; apply proof_irrelevance.
 Qed.
 Next Obligation.
-  rewrite mlSortOfTerm_mlSort2Sort with (i:=mlTermIn2mlTermSortIn _ h1).
-  rewrite mlSortOfTerm_mlSort2Sort with (i:=mlTermIn2mlTermSortIn _ h2).
-  generalize (mlTermIn2mlTermSortIn t1 h1); rewrite e; intro.
+  rewrite mlSortOfTerm_mlSort2Sort with (i:=termIn2termSortIn _ h1).
+  rewrite mlSortOfTerm_mlSort2Sort with (i:=termIn2termSortIn _ h2).
+  generalize (termIn2termSortIn t1 h1); rewrite e; intro.
   f_equal; apply proof_irrelevance.
 Qed.
 
 Lemma  mlEx_Var_In: forall {v b},
-  incl (mlFormulaIds (MLEx v b)) (mlModelIds mdl) ->
-    In v (mlAllVariables mdl).
+  incl (mlUtils.formulaIds (api.Exists v b)) (mlUtils.modelIds mdl) ->
+    In v (mlUtils.mlAllVariables mdl).
 Proof.
   simpl; intros.
   apply incl_cons_inv in H; apply proj2 in H.
   apply incl_cons_inv in H; apply proj1 in H.
-  unfold mlAllVariables.
-  apply (imap_filter_In_intro _ _ isMLVarDec (mlModelIds mdl)
-   (fun (v0 : mlIdent) (h1 : isMLVar v0) (_ : In v0 (mlModelIds mdl))
-      => getMLVar v0 h1) (MLV _) I H).
+  unfold mlUtils.mlAllVariables.
+  apply (imap_filter_In_intro _ _ api.isVarDec (mlUtils.modelIds mdl)
+   (fun (v0 : api.mlIdent) (h1 : api.isVar v0) (_ : In v0 (mlUtils.modelIds mdl))
+      => api.getVar v0 h1) (api.MLV _) I H).
 Qed.
 
 Lemma  mlEx_bdy_incl: forall {v b},
-  incl (mlFormulaIds (MLEx v b)) (mlModelIds mdl) ->
-    incl (mlFormulaIds b) (mlModelIds mdl).
+  incl (mlUtils.formulaIds (api.Exists v b)) (mlUtils.modelIds mdl) ->
+    incl (mlUtils.formulaIds b) (mlUtils.modelIds mdl).
 Proof.
   simpl; intros.
   apply incl_cons_inv in H; apply proj2 in H.
@@ -280,21 +277,21 @@ Proof.
 Qed.
 
 Lemma  mlAll_Var_In: forall {v b},
-  incl (mlFormulaIds (MLAll v b)) (mlModelIds mdl) ->
-    In v (mlAllVariables mdl).
+  incl (mlUtils.formulaIds (api.All v b)) (mlUtils.modelIds mdl) ->
+    In v (mlUtils.mlAllVariables mdl).
 Proof.
   simpl; intros.
   apply incl_cons_inv in H; apply proj2 in H.
   apply incl_cons_inv in H; apply proj1 in H.
-  unfold mlAllVariables.
-  apply (imap_filter_In_intro _ _ isMLVarDec (mlModelIds mdl)
-   (fun (v0 : mlIdent) (h1 : isMLVar v0) (_ : In v0 (mlModelIds mdl))
-      => getMLVar v0 h1) (MLV _) I H).
+  unfold mlUtils.mlAllVariables.
+  apply (imap_filter_In_intro _ _ api.isVarDec (mlUtils.modelIds mdl)
+   (fun (v0 : api.mlIdent) (h1 : api.isVar v0) (_ : In v0 (mlUtils.modelIds mdl))
+      => api.getVar v0 h1) (api.MLV _) I H).
 Qed.
 
 Lemma  mlAll_bdy_incl: forall {v b},
-  incl (mlFormulaIds (MLAll v b)) (mlModelIds mdl) ->
-    incl (mlFormulaIds b) (mlModelIds mdl).
+  incl (mlUtils.formulaIds (api.All v b)) (mlUtils.modelIds mdl) ->
+    incl (mlUtils.formulaIds b) (mlUtils.modelIds mdl).
 Proof.
   simpl; intros.
   apply incl_cons_inv in H; apply proj2 in H.
@@ -302,21 +299,21 @@ Proof.
   apply H.
 Qed.
 
-Fixpoint mlFormula2formula f: List.incl (mlFormulaIds f) (mlModelIds mdl) -> formula coqSig := 
-  match f return List.incl (mlFormulaIds f) (mlModelIds mdl) -> formula coqSig with
-    MLFTrue => fun h => FTrue coqSig
-  | MLFFalse => fun h => FFalse coqSig
-  | MLAtom a => mlAtom2Atom a
-  | MLAnd f1 f2 => fun h => 
+Fixpoint formula2formula f: List.incl (mlUtils.formulaIds f) (mlUtils.modelIds mdl) -> foltl.formula coqSig := 
+  match f return List.incl (mlUtils.formulaIds f) (mlUtils.modelIds mdl) -> foltl.formula coqSig with
+    api.True => fun h => foltl.FTrue coqSig
+  | api.False => fun h => foltl.FFalse coqSig
+  | api.Lit a => literal2Atom a
+  | api.And f1 f2 => fun h => 
     let (h1,h2) := incl_app_inv _ _ h in
-    And coqSig (mlFormula2formula f1 h1) (mlFormula2formula f2 h2)
-  | MLOr f1 f2 => fun h => 
+    foltl.And coqSig (formula2formula f1 h1) (formula2formula f2 h2)
+  | api.Or f1 f2 => fun h => 
     let (h1,h2) := incl_app_inv _ _ h in
-    Or coqSig (mlFormula2formula f1 h1) (mlFormula2formula f2 h2)
-  | MLEx v b => fun h => Ex coqSig _ (mlVar2Var v (mlEx_Var_In h)) (mlFormula2formula b (mlEx_bdy_incl h))
-  | MLAll v b => fun h => All coqSig _ (mlVar2Var v (mlAll_Var_In h)) (mlFormula2formula b (mlAll_bdy_incl h))
-  | MLF f' => fun h => F coqSig (mlFormula2formula f' h)
-  | MLG f' => fun h => G coqSig (mlFormula2formula f' h)
+    foltl.Or coqSig (formula2formula f1 h1) (formula2formula f2 h2)
+  | api.Exists v b => fun h => foltl.Ex coqSig _ (mlVar2Var v (mlEx_Var_In h)) (formula2formula b (mlEx_bdy_incl h))
+  | api.All v b => fun h => foltl.All coqSig _ (mlVar2Var v (mlAll_Var_In h)) (formula2formula b (mlAll_bdy_incl h))
+  | api.F f' => fun h => foltl.F coqSig (formula2formula f' h)
+  | api.G f' => fun h => foltl.G coqSig (formula2formula f' h)
   end.
 
 End ML2Coq.
