coq/coq2ml.v
@@ -1,7 +1,7 @@
 Require Import String.
 
 Require Import foltl.
-Require Import api.
+Require api.
 Require Import dec.
 Require Import finite.
 Require utils.
@@ -11,53 +11,53 @@ Section COQ2ML.
   Context {Ts: Type} {Tv: Ts->Type} {Tc: Ts->Type} {Tp: Type}.
   Variable Sg: @Sig Ts Tv Tc Tp.
 
-  Variable sort2ml: Sort (Sig:=Sg) -> mlSort.
+  Variable sort2ml: Sort (Sig:=Sg) -> api.mlSort.
   Variable varName : forall {s: Sort (Sig:=Sg)}, variable (Sig:=Sg) s -> string.
   Variable cstName : forall {s: Sort (Sig:=Sg)}, constant (Sig:=Sg) s -> string.
   Variable relName : predicate (Sig:=Sg) -> string.
 
-  Definition var2ml {s: Sort (Sig:=Sg)} (v: variable (Sig:=Sg) s) : mlVariable := {|
-    mlVarName := varName v;
-    mlVarSort := sort2ml s;
+  Definition var2ml {s: Sort (Sig:=Sg)} (v: variable (Sig:=Sg) s) : api.variable := {|
+    api.var_name := varName v;
+    api.var_sort := sort2ml s;
   |}.
 
-  Definition cst2ml {s: Sort (Sig:=Sg)} (c: constant (Sig:=Sg) s) : mlConstant := {|
-    mlCstName := cstName c;
-    mlCstSort := sort2ml s;
+  Definition cst2ml {s: Sort (Sig:=Sg)} (c: constant (Sig:=Sg) s) : api.constant := {|
+    api.cst_name := cstName c;
+    api.cst_sort := sort2ml s;
   |}.
 
   Definition rel2ml (r: predicate (Sig:=Sg)) : string := relName r.
 
   Definition tm2ml {s} (tm: term Sg s) :=
     match tm with
-      Var _ _ v => MLVar (var2ml v)
-    | Cst _ _ c => MLCst (cst2ml c)
+      Var _ _ v => api.Var (var2ml v)
+    | Cst _ _ c => api.Cst (cst2ml c)
     end.
 
-  Definition lt2ml (l: literal Sg) :=
+  Definition lt2ml sgn (l: literal Sg): api.literal :=
     match l with
-      PApp _ x p a => MLPApp x (rel2ml p) (utils.fmap (fun i => tm2ml (a i)))
+      PApp _ x p a => sgn x (rel2ml p) (utils.fmap (fun i => tm2ml (a i)))
     end.
 
   Definition at2ml (a: atom Sg) :=
   match a with
-    Literal _ l => MLLiteral (lt2ml l)
-  | NLiteral _ l => MLNLiteral (lt2ml l)
-  | Eq _ s t1 t2 => MLEq (tm2ml t1) (tm2ml t2)
-  | NEq _ s t1 t2 => MLNEq (tm2ml t1) (tm2ml t2)
+    Literal _ l => lt2ml api.Pos_app l
+  | NLiteral _ l => lt2ml api.Neg_app l
+  | Eq _ s t1 t2 => api.Eq (tm2ml t1) (tm2ml t2)
+  | NEq _ s t1 t2 => api.Not_eq (tm2ml t1) (tm2ml t2)
   end.
 
   Fixpoint fm2ml (f: formula Sg) :=
   match f with
-    | FTrue _ => MLFTrue
-    | FFalse _ => MLFFalse
-    | Atom _ a => MLAtom (at2ml a)
-    | And _ f1 f2 => MLAnd (fm2ml f1) (fm2ml f2)
-    | Or _ f1 f2 => MLOr (fm2ml f1) (fm2ml f2)
-    | Ex _ s v f => MLEx (var2ml v) (fm2ml f)
-    | All _ s v f => MLAll (var2ml v) (fm2ml f)
-    | F _ f => MLF(fm2ml f)
-    | G _ f => MLG (fm2ml f)
+    | FTrue _ => api.True
+    | FFalse _ => api.False
+    | Atom _ a => api.Lit (at2ml a)
+    | And _ f1 f2 => api.And (fm2ml f1) (fm2ml f2)
+    | Or _ f1 f2 => api.Or (fm2ml f1) (fm2ml f2)
+    | Ex _ s v f => api.Exists (var2ml v) (fm2ml f)
+    | All _ s v f => api.All (var2ml v) (fm2ml f)
+    | F _ f => api.F (fm2ml f)
+    | G _ f => api.G (fm2ml f)
   end.
 
 End COQ2ML.
